Prove a triple for ADD

Hoare.thy
@@ -29,10 +29,10 @@ datatype state_element =
   | SentDataElm "nat * byte" (* position, content.  Considering making position an int *)
   | ExtProgramSizeElm "address * int" (* address, size.  Considering making size an int *)
   | ExtProgramElm "address * nat * byte" (* address, position, byte.  Considering making position an int *)
-  | ContractActionElm "contract_action option" (* None indicates continued execution *)
+  | ContractActionElm "contract_action" (* None indicates continued execution *)
 
 definition contract_action_as_set :: "contract_action \<Rightarrow> state_element set"
-  where "contract_action_as_set act == { ContractActionElm (Some act) }"
+  where "contract_action_as_set act == { ContractActionElm act }"
 
 definition memory_as_set :: "memory \<Rightarrow> state_element set"
   where
@@ -49,7 +49,7 @@ definition balance_as_set :: "(address \<Rightarrow> w256) \<Rightarrow> state_e
 definition stack_as_set :: "w256 list \<Rightarrow> state_element set"
   where
     "stack_as_set s == { StackHeightElm (length s) } \<union>
-                       { StackElm (idx, v) | idx v. s ! idx = v }"
+                       { StackElm (idx, v) | idx v. idx < length s \<and> (rev s) ! idx = v }"
 
 definition data_sent_as_set :: "byte list \<Rightarrow> state_element set"
   where
@@ -94,6 +94,7 @@ definition variable_ctx_as_set :: "variable_ctx \<Rightarrow> state_element set"
       , OriginElm (vctx_origin v)
       , BlockInfoElm (vctx_block v)
       , GasElm (vctx_gas v)
+      , PcElm (vctx_pc v)
       }"
 
 definition contexts_as_set :: "variable_ctx \<Rightarrow> constant_ctx \<Rightarrow> state_element set"
@@ -104,9 +105,14 @@ definition contexts_as_set :: "variable_ctx \<Rightarrow> constant_ctx \<Rightar
 (* From Magnus Myreen's thesis, Section 3.3 *)
 definition sep :: "(state_element set \<Rightarrow> bool) \<Rightarrow> (state_element set \<Rightarrow> bool) \<Rightarrow> state_element set \<Rightarrow> bool"
   where
-    "sep p q s == \<exists> u v. p u \<and> q v \<and> u \<union> v = s \<and> u \<inter> v = {} "
+    "sep p q == (\<lambda> s. \<exists> u v. p u \<and> q v \<and> u \<union> v = s \<and> u \<inter> v = {})"
 
 notation sep (infixr "**" 60)
+
+lemma sep_assoc [simp] : "((p ** q) ** r) s = (p ** q ** r) s"
+  apply(auto simp add: sep_def)
+  apply(rule_tac x = "ua" in exI; auto)
+done
 
 definition emp :: "state_element set \<Rightarrow> bool"
   where
@@ -126,6 +132,14 @@ definition stack :: "nat \<Rightarrow> w256 \<Rightarrow> state_element set \<Ri
   where
     "stack pos v s == (s = {StackElm (pos, v)})"
 
+definition program_counter :: "int \<Rightarrow> state_element set \<Rightarrow> bool"
+  where
+    "program_counter pos s == s = {PcElm pos}"
+
+definition gas_pred :: "int \<Rightarrow> state_element set \<Rightarrow> bool"
+  where
+    "gas_pred g s == s = {GasElm g}"
+
 (* memory8, memory, calldata, and storage should be added here *)
 
 lemma stack_sound0 :
@@ -134,14 +148,14 @@ apply(auto simp add: sep_def stack_def)
 done
 
 lemma stack_sound1 :
-  "StackElm (pos, w) \<in> contexts_as_set var con \<Longrightarrow> vctx_stack var ! pos = w"
+  "StackElm (pos, w) \<in> contexts_as_set var con \<Longrightarrow> rev (vctx_stack var) ! pos = w"
   apply(simp add: contexts_as_set_def variable_ctx_as_set_def constant_ctx_as_set_def
       stack_as_set_def memory_as_set_def
       balance_as_set_def storage_as_set_def log_as_set_def program_as_set_def)
   done
 
 lemma stack_sem :
-  "(stack pos w ** p) (contexts_as_set var con) \<Longrightarrow> vctx_stack var ! pos = w"
+  "(stack pos w ** p) (contexts_as_set var con) \<Longrightarrow> rev (vctx_stack var) ! pos = w"
   apply(drule stack_sound0)
   apply(drule stack_sound1)
   apply(simp)
@@ -151,7 +165,7 @@ definition program_result_as_set :: "constant_ctx \<Rightarrow> program_result \
   where
     "program_result_as_set c rslt =
         ( case rslt of
-          ProgramStepRunOut v \<Rightarrow> contexts_as_set v c \<union> { ContractActionElm None }
+          ProgramStepRunOut v \<Rightarrow> contexts_as_set v c
         | ProgramToEnvironment act st bal _ logs None \<Rightarrow>
           constant_ctx_as_set c \<union>
           contract_action_as_set act \<union> storage_as_set st \<union> balance_as_set bal \<union> log_as_set logs
@@ -183,8 +197,173 @@ where
   "triple pre insts post ==
     \<forall> va_ctx co_ctx rest. no_assertion co_ctx \<longrightarrow> recent_protocol va_ctx \<longrightarrow>
        (pre ** code insts ** rest) (contexts_as_set va_ctx co_ctx) \<longrightarrow>
-       (\<exists> k. (post ** code insts ** rest) (program_result_as_set co_ctx (program_sem va_ctx co_ctx k (nat k))))"
+       (\<exists> k. (post ** code insts ** rest) (program_result_as_set co_ctx (program_sem va_ctx co_ctx k)))"
 
+lemma no_assertion_pass [simp] : "no_assertion co_ctx \<Longrightarrow> check_annotations v co_ctx"
+apply(simp add: no_assertion_def check_annotations_def)
+done
+    
+lemma pure_sep [simp] : "(\<langle> b \<rangle> ** rest) s = (b \<and> rest s)"
+apply(simp add: sep_def pure_def emp_def)
+done
+
+lemma stack_height_sep [simp] : "(stack_height h ** rest) s =
+  (StackHeightElm h \<in> s \<and> rest (s - {StackHeightElm h})) "
+apply(auto simp add: sep_def stack_height_def)
+done
+
+lemma stack_sep [simp] : "(stack p w ** rest) s =
+  (StackElm (p, w) \<in> s \<and> rest (s - {StackElm (p, w)}))"
+apply(auto simp add: sep_def stack_def)
+done
+
+lemma program_counter_sep [simp] : "(program_counter w ** rest) s =
+  (PcElm w \<in> s \<and> rest (s - {PcElm w}))"
+apply(auto simp add: sep_def program_counter_def)
+done
+
+lemma code_sep [simp] : "(code pairs ** rest) s =
+  ({ CodeElm(pos, i) | pos i. (pos, i) \<in> pairs } \<subseteq> s \<and> (rest (s - { CodeElm(pos, i) | pos i. (pos, i) \<in> pairs })))"
+  apply(auto simp add: sep_def code_def)
+  apply(simp add: Set.Un_Diff)
+  by (simp add: Diff_triv inf_commute)
+
+lemma gas_pred_sep [simp] : "(gas_pred g ** rest) s =
+  ( GasElm g \<in> s \<and> rest (s - { GasElm g }) )"
+  apply(auto simp add: sep_def gas_pred_def)
+done
+
+lemma stackHeightElmEquiv [simp] : "StackHeightElm h \<in> contexts_as_set v c =
+  (length (vctx_stack v) = h)
+  "
+apply(auto simp add: contexts_as_set_def constant_ctx_as_set_def variable_ctx_as_set_def
+      program_as_set_def stack_as_set_def memory_as_set_def storage_as_set_def
+      balance_as_set_def log_as_set_def)
+  done
+
+lemma stackElmEquiv [simp] : "StackElm (pos, w) \<in> contexts_as_set v c =
+  (pos < length (vctx_stack v) \<and> rev (vctx_stack v) ! pos = w)"
+apply(auto simp add: contexts_as_set_def constant_ctx_as_set_def variable_ctx_as_set_def
+      program_as_set_def stack_as_set_def memory_as_set_def storage_as_set_def
+      balance_as_set_def log_as_set_def)
+done
+
+lemma pcElmEquiv [simp] : "PcElm k \<in> contexts_as_set va_ctx co_ctx =
+  (vctx_pc va_ctx = k)"
+apply(auto simp add: contexts_as_set_def constant_ctx_as_set_def variable_ctx_as_set_def
+      program_as_set_def stack_as_set_def memory_as_set_def storage_as_set_def
+      balance_as_set_def log_as_set_def)
+done
+
+lemma gasElmEquiv [simp] : "GasElm g \<in> contexts_as_set va_ctx co_ctx =
+  (vctx_gas va_ctx = g)"
+apply(auto simp add: contexts_as_set_def constant_ctx_as_set_def variable_ctx_as_set_def
+      program_as_set_def stack_as_set_def memory_as_set_def storage_as_set_def
+      balance_as_set_def log_as_set_def)
+done
+
+lemma codeElmEquiv [simp] :
+  "CodeElm (pos, i) \<in> contexts_as_set va_ctx co_ctx =
+   ((program_content (cctx_program co_ctx) pos = Some i) \<or>
+   (program_content (cctx_program co_ctx) pos = None) \<and> i = Misc STOP)"
+apply(auto simp add: contexts_as_set_def constant_ctx_as_set_def variable_ctx_as_set_def
+      program_as_set_def stack_as_set_def memory_as_set_def storage_as_set_def
+      balance_as_set_def log_as_set_def)
+done
+
+lemma insert_minus : "a \<noteq> b \<Longrightarrow> insert a s - { b } = insert a (s - {b})"
+  apply(simp add: insert_Diff_if)
+  done
+
+lemma pred_functional : "p (s :: state_element set) \<Longrightarrow> s = t \<Longrightarrow> p t"
+apply(auto)
+done
+
+lemma insert_functional : "e = f \<Longrightarrow> s = t \<Longrightarrow> insert e s = insert f t"
+  apply(auto)
+  done
+
+lemma lookup_over [simp] : "(rev lista @ (aa # l)) ! length lista = aa"
+	by (metis length_rev nth_append_length)
+
+lemma lookup_over1 [simp] : "(rev lista @ (w # a # l)) ! Suc (length lista) = a"
+(* sledgehammer *)
+	by (metis add.left_neutral append.assoc append_Nil2 length_append length_rev list.size(3) list.size(4) nth_append_length plus_nat.simps(2) rev.simps(2) rev_append rev_rev_ident)
+
+lemma short_match [simp] :
+  "idx < length lista \<Longrightarrow> (rev lista @ l) ! idx = (rev lista @ m) ! idx"
+(* sledgehammer *)
+	by (simp add: nth_append)
+		
+declare memory_as_set_def [simp]
+  storage_as_set_def [simp]
+  log_as_set_def [simp]
+  balance_as_set_def [simp]
+  
+lemma add_triple : "triple (\<langle> h \<le> 1023 \<and> g \<ge> Gverylow \<rangle> **
+                            stack_height (h + 2) **
+                            stack (h + 1) v **
+                            stack h w **
+                            program_counter k **
+                            gas_pred g
+                           )
+                           {(k, Arith ADD)}
+                           (stack_height (h + 1) **
+                            stack h (v + w) **
+                            program_counter (k + 1) **
+                            gas_pred (g - Gverylow)
+                            )"
+apply(auto simp add: triple_def)
+apply(rule_tac x = "1" in exI)
+apply(simp add: program_sem.simps vctx_next_instruction_def instruction_sem_def check_resources_def
+      inst_stack_numbers.simps arith_inst_numbers.simps predict_gas_def C_def Cmem_def
+      Gmemory_def new_memory_consumption.simps thirdComponentOfC.simps
+      vctx_next_instruction_default_def stack_2_1_op_def)
+apply(case_tac "vctx_stack va_ctx"; simp)
+apply(case_tac list; simp)
+apply(auto simp add: subtract_gas.simps strict_if_def program_sem.simps program_result_as_set_def
+      vctx_advance_pc_def vctx_next_instruction_def inst_size_def inst_code.simps
+      contexts_as_set_def constant_ctx_as_set_def variable_ctx_as_set_def stack_as_set_def
+      program_as_set_def)
+apply(simp add: insert_Diff_if)
+apply(rule pred_functional)
+ apply(simp)
+apply(rule insert_functional; blast?)
+apply(rule insert_functional; blast?)
+apply(rule insert_functional; blast?)
+apply(rule insert_functional; blast?)
+apply(rule insert_functional; blast?)
+apply(rule insert_functional; blast?)
+apply(rule Set.equalityI)
+ apply(clarify)
+ apply(simp)
+ apply(drule disjE; simp)
+ apply(drule disjE; simp?)
+  apply(blast)
+ apply(drule disjE; simp?)
+  defer
+  apply(clarify)
+  apply(simp)
+  apply(case_tac "idx \<ge> length lista"; simp)
+  apply(case_tac "idx = Suc (length lista)"; simp)
+ apply(clarify)
+ apply(simp)
+ apply(drule disjE; simp?)
+  apply(drule disjE; simp?)
+   apply(blast)
+  apply(drule disjE; simp?)
+   defer
+   apply(clarify)
+   apply(simp)
+   apply(case_tac "idx = (length lista)"; simp)
+  apply(drule disjE; simp?)
+   apply(blast)
+  apply(drule disjE; simp?)
+ apply(clarify)
+ apply(simp)
+apply(clarify)
+apply(simp)
+done
 
 (* Some rules about this if-then-else should be derivable. *)
 
